Refactor code

dafny/abstract-interpreter/SimpleVerifierAnalysis.dfy
@@ -1,18 +1,21 @@
 include "SimpleVerifier.dfy"
 include "BoundedInts.dfy"
+include "ConcreteExecution.dfy"
+include "helpers.dfy"
 
 module SimpleVerifierAnalysis {
   import opened Lang
   import opened E = ConcreteEval
   import opened AbstractEval
+  import opened ConcreteExecution
   import opened Ints
   import opened BoundedInts
   import opened AbstractEvalProof
+  import opened helpers
 
-  datatype PathState = PathState(state: E.State, pc: int)
+  datatype AbstractPathState = AbstractPathState(state: AbstractState, pc: nat, branch_pcs: seq<nat>)
 
-  datatype AbstractPathState = AbstractPathState(state: AbstractState, pc: int, branch_pcs: seq<int>)
-
+  // Expected to satisfy stmt_step(path[i].state, path[i].pc) ~> (path[i + 1].state)
   datatype AbstractPath = AbstractPath(path: seq<AbstractPathState>)
   datatype AnalysisResult = AnalysisResult(paths: seq<AbstractPath>)
 
@@ -21,154 +24,18 @@ module SimpleVerifierAnalysis {
 
   datatype InstructionType = BranchInstruction | FunctionExit
 
-  datatype ConcretePath = ConcretePath(path: seq<PathState>)
-
-  predicate state_equal(s1: E.State, s2: E.State) {
-    forall r : Reg :: s1(r) == s2(r)
-  }
-
-  predicate stmt_step_valid(prog: Program, pc: int, env: E.State, pc': int, env': E.State)
-    requires 0 <= pc <= |prog.stmts|
-    requires 0 <= pc' <= |prog.stmts|
-    requires (pc == |prog.stmts|) ==> (pc' == |prog.stmts|)
-  {
-    if pc == |prog.stmts| then
-      true
-    else
-      var stmt := prog.stmts[pc];
-      match E.stmt_step(env, stmt) {
-        case Some((env'', offset)) =>
-          (pc + offset == pc') && state_equal(env', env'')
-        case None => false
-      }
-  }
-
-  // TODO: Write predicate for a valid path
-  // TODO: Relate 2 states at the same time
-  predicate path_valid(prog: Program, path_states: seq<PathState>)
-  {
-    if |path_states| <= 1 then
-      true
-    else
-    if path_states[0].pc < 0 || path_states[0].pc > |prog.stmts| then
-      false
-    else if path_states[0].pc == |prog.stmts| then
-      (path_states[1].pc == |prog.stmts|) && path_valid(prog, path_states[1..])
-    else
-      var stmt := prog.stmts[path_states[0].pc];
-      match E.stmt_step(path_states[0].state, stmt) {
-        case Some((env', offset)) =>
-          ((path_states[0].pc + offset) == path_states[1].pc) && path_valid(prog, path_states[1..])
-        case None => false
-      }
-  }
-
-  method m1(prog: Program, a: seq<PathState>, b: seq<PathState>)
-    requires |a| > 0
-  {
-    assert a == [a[0]] + a[1..];
-    assert bridges(prog, [a[0]], a[1..]) && path_valid(prog, a[1..]) <==> path_valid(prog, a);
-  }
-
-
-  lemma ValidPathConcat(prog: Program, path_states: seq<PathState>)
-    requires |path_states| > 0
-    requires path_valid(prog, path_states)
-    ensures forall i :: 0 <= i < |path_states| - 1 ==> path_valid(prog, [path_states[i], path_states[i + 1]])
-  {
-
-  }
-
-  predicate bridges(prog: Program, a: seq<PathState>, b: seq<PathState>)
-  {
-    if b == [] || a == [] then
-      true
-    else
-    if a[|a| - 1].pc < 0 || a[|a| - 1].pc > |prog.stmts| then
-      false
-    else if a[|a| - 1].pc == |prog.stmts| then
-      b[0].pc == |prog.stmts| //&& path_valid(prog, b)
-    else
-      var stmt := prog.stmts[a[|a| - 1].pc];
-      match E.stmt_step(a[|a| - 1].state, stmt) {
-        case Some((env', offset)) =>
-          ((a[|a| - 1].pc + offset) == b[0].pc) //&& path_valid(prog, b)
-        case None => false
-      }
-  }
-
-  lemma ValidPathsConcat(prog: Program, a: seq<PathState>, b: seq<PathState>)
-    ensures path_valid(prog, a + b) == (path_valid(prog, a) && bridges(prog, a, b) && path_valid(prog, b))
-  {
-    if a == [] {
-      assert a + b == b;
-      assert bridges(prog, a, b);
-      assert path_valid(prog, a);
-      assert path_valid(prog, a + b) == (path_valid(prog, a) && bridges(prog, a, b) && path_valid(prog, b));
-    } else if b == [] {
-      assert a + b == a;
-      assert bridges(prog, a, b);
-      assert path_valid(prog, b);
-      assert path_valid(prog, a + b) == (path_valid(prog, a) && bridges(prog, a, b) && path_valid(prog, b));
-    } else {
-      assert |a + b| >= 2;
-      assert a + b == [a[0]] + (a[1..] + b);
-      assert path_valid(prog, a + b) == path_valid(prog, [a[0]] + (a[1..] + b));
-    }
-  }
-
-  lemma PathBridgeConcat(prog: Program, a: seq<PathState>, bridge: PathState, b: seq<PathState>)
-    ensures path_valid(prog, a + [bridge]) && bridges(prog, a + [bridge], b) && path_valid(prog, [bridge] + b) <==> path_valid(prog, a + [bridge] + b)
-  {
-    ValidPathsConcat(prog, a, [bridge]);
-    assert path_valid(prog, a + [bridge]) == (path_valid(prog, a) && bridges(prog, a, [bridge]) && path_valid(prog, [bridge]));
-
-    ValidPathsConcat(prog, [bridge], b);
-    assert path_valid(prog, [bridge] + b) == (path_valid(prog, [bridge]) && bridges(prog, [bridge], b) && path_valid(prog, b));
-
-    //ValidPathsConcat(prog, a + [bridge], b);
-    assert a + ([bridge] + b) == (a + [bridge]) + b ;
-    ValidPathsConcat(prog, a + [bridge], b);
-    //assert path_valid(prog, a + [bridge] + b) == path_valid(prog, a + [bridge]) && bridges(prog, a + [bridge], b) && path_valid(prog, b);
-
-    assert (a + [bridge] + b) == (a + ([bridge] + b));
-    assert path_valid(prog, a + [bridge]) && path_valid(prog, [bridge] + b) ==> path_valid(prog, a) && path_valid(prog, b) && bridges(prog, a, [bridge]) && bridges(prog, [bridge], b);
-  }
-
   function init_abs_reg_state(r: Reg): Val {
     //TODO: Maybe this should be (0, U64_MAX)
     //TODO: All registers are unconstrained
     Interval(0, U64_MAX as int)
   }
 
-  function init_conc_reg_state(r: Reg): u32 {
-    0
-  }
-
   function initial_abstract_state(stmt: Stmt): AbstractPathState {
     AbstractPathState(AbstractState(init_abs_reg_state), 0, [])
   }
 
-  function initial_concrete_state(stmt: Stmt): PathState {
-    PathState(init_conc_reg_state, 0)
-  }
-
   function push_stack(stack: seq<AbstractPathState>, new_state: AbstractPathState): seq<AbstractPathState> {
     stack + [new_state]
-  }
-
-  function backtrack_stack(stack: seq<AbstractPathState>, concrete_stack: seq<PathState>): (seq<AbstractPathState>, seq<PathState>)
-    ensures |backtrack_stack(stack, concrete_stack).0| > 0 ==> |backtrack_stack(stack, concrete_stack).0[|backtrack_stack(stack, concrete_stack).0| - 1].branch_pcs| > 0
-    ensures |stack| == |concrete_stack| ==> |backtrack_stack(stack, concrete_stack).0| == |backtrack_stack(stack, concrete_stack).1|
-    ensures |stack| == |concrete_stack| && (forall j :: 0 <= j < |stack| ==> path_state_included(concrete_stack[j], stack[j]))
-            ==> (forall i :: 0 <= i < |backtrack_stack(stack, concrete_stack).1| ==> path_state_included(backtrack_stack(stack, concrete_stack).1[i], backtrack_stack(stack, concrete_stack).0[i]))
-  {
-    if |stack| == 0 || |concrete_stack| == 0 then
-      ([], [])
-    else if |stack[|stack| - 1].branch_pcs| > 0 then
-      (stack, concrete_stack)
-    else
-      backtrack_stack(stack[..|stack| - 1], concrete_stack[..|concrete_stack| - 1])
   }
 
   predicate reg_included(c_v: u32, v: Val) {
@@ -179,146 +46,6 @@ module SimpleVerifierAnalysis {
     forall r: Reg :: reg_included(env(r), abs.rs(r))
   }
 
-  predicate path_state_included(path_state: PathState, abs_path_state: AbstractPathState) {
-    (path_state.pc == abs_path_state.pc) &&
-    (state_included(path_state.state, abs_path_state.state))
-  }
-
-  method explore_abstract_paths(prog: Program, fuel: int, init_conc_state: PathState, init_abstract_state: AbstractPathState)
-    requires fuel >= 0
-    requires |prog.stmts| > 0
-    requires path_state_included(init_conc_state, init_abstract_state)
-  {
-    var stack : seq<AbstractPathState> := [init_abstract_state];
-    var fuel := fuel;
-    var concrete_stack : seq<PathState> := [init_conc_state];
-
-    assert (path_state_included(concrete_stack[0], stack[0]));
-    assert |concrete_stack| == |stack|;
-    assert path_valid(prog, concrete_stack);
-
-    while fuel > 0 && |stack| > 0
-      invariant |concrete_stack| == |stack|
-      // Proving that the actual execution is a subset of the static path wrt all taken branches
-      invariant forall i :: 0 <= i < |stack| ==> path_state_included(concrete_stack[i], stack[i])
-      //invariant path_valid(prog, concrete_stack);
-    {
-      // Pop topmost state from the abstract path stack
-      var cur_state := stack[|stack| - 1];
-      var cur_pc := cur_state.pc;
-      stack := stack[..|stack| - 1];
-
-      // Pop topmost state from the concrete path stack
-      var cur_conc_state := concrete_stack[|concrete_stack| - 1];
-      var cur_conc_pc := cur_conc_state.pc;
-      concrete_stack := concrete_stack[..|concrete_stack| - 1];
-      //assert path_valid(prog, concrete_stack);
-
-      if cur_pc < 0 || cur_pc > |prog.stmts| {
-        // We should never encounter this
-        break;
-      }
-
-      if cur_pc == |prog.stmts| {
-        // We hit the end of this concrete execution
-
-        // Commenting out backtracking code
-        // We hit the end of the subroutine
-        // Backtrack till an abstract state with |branch_pcs| > 0 and
-        // explore one of those paths
-        /*var s := backtrack_stack(stack, concrete_stack);
-        stack := s.0;
-        concrete_stack := s.1;
-
-        if |stack| > 0 {
-          var last_state := stack[|stack| - 1].state;
-          var last_pc := stack[|stack| - 1].pc;
-          var last_branches := stack[|stack| - 1].branch_pcs;
-
-          var new_pc := stack[|stack| - 1].branch_pcs[0];
-
-          var new_branch_state := AbstractPathState(last_state, last_pc, last_branches[1..]);
-          stack := stack[|stack| - 1 := new_branch_state];
-
-          var new_expl_state := AbstractPathState(last_state, new_pc, []);
-          stack := push_stack(stack, new_expl_state);
-
-          var last_conc_state := concrete_stack[|concrete_stack| - 1].state;
-          var last_conc_pc := concrete_stack[|concrete_stack| - 1].pc;
-          concrete_stack := concrete_stack + [PathState(last_conc_state, new_pc)];
-
-        }
-        fuel := fuel - 1;
-        continue;*/
-        break;
-      }
-
-      // Continue exploring the path
-      var cur_stmt := prog.stmts[cur_state.pc];
-      var conc_step := stmt_step(cur_conc_state.state, cur_stmt);
-
-      if conc_step.None? {
-        // Invalid Execution Path
-        break;
-      }
-
-      assert cur_conc_pc == cur_pc;
-
-      match cur_stmt {
-        case Assign(r, e) => {
-
-          var v := AbstractEval.expr_eval(cur_state.state, e);
-          var new_state := AbstractEval.update_state(cur_state.state, r, v);
-          // We rewrite the branches array when this state is being popped off
-          // Iff it is a branch instruction
-          var new_abs_state := AbstractPathState(new_state, cur_pc + 1, []);
-          stack := push_stack(stack, new_abs_state);
-
-          assert conc_step.v.1 == 1;
-          var new_conc_state := PathState(conc_step.v.0, cur_pc + conc_step.v.1);
-          concrete_stack := concrete_stack + [new_conc_state];
-
-          assert (path_state_included(new_conc_state, new_abs_state));
-          assert path_state_included(concrete_stack[|concrete_stack| - 1], stack[|stack| - 1]);
-
-          assert bridges(prog, [cur_conc_state], [new_conc_state]);
-          assert bridges(prog, concrete_stack + [cur_conc_state], [new_conc_state]);
-        }
-
-        case JmpZero(r, offset) => {
-          // Copied from AbstractEval.stmt_eval
-          // imprecise analysis: we don't try to prove that this jump is or isn't taken
-          var fall_through := AbstractPathState(cur_state.state, cur_pc + 1, []);
-          var jmp_targ := AbstractPathState(cur_state.state, cur_pc + offset as int, []);
-          var jmp_state := AbstractPathState(cur_state.state, cur_pc, []);
-
-          var jmp_conc_state := PathState(cur_conc_state.state, cur_pc);
-          var jmp_conc_targ := PathState(cur_conc_state.state, cur_pc + offset as int);
-          var conc_fall_through := PathState(cur_conc_state.state, cur_pc + 1);
-
-          assert (path_state_included(jmp_conc_targ, jmp_targ));
-          assert (path_state_included(conc_fall_through, fall_through));
-
-          // We are interested in only the actual branch that is taken
-          if conc_step.v.1 == offset as int {
-            // Explore the target branch
-            stack := push_stack(push_stack(stack, jmp_state), jmp_targ);
-            concrete_stack := concrete_stack + [jmp_conc_state] + [jmp_conc_targ];
-            assert(cur_conc_state == jmp_conc_state);
-            assert (path_valid(prog, [jmp_conc_state, jmp_conc_targ]));
-          } else {
-            stack := push_stack(push_stack(stack, jmp_state), fall_through);
-            concrete_stack := concrete_stack + [jmp_conc_state] + [conc_fall_through];
-            assert (path_valid(prog, [jmp_conc_state, conc_fall_through]));
-          }
-          assert path_state_included(concrete_stack[|concrete_stack| - 1], stack[|stack| - 1]);
-        }
-      }
-
-      fuel := fuel - 1;
-    }
-  }
-
   predicate programWellFormed(prog: Program) {
     true
   }
@@ -327,82 +54,77 @@ module SimpleVerifierAnalysis {
     AbstractPath(absPath.path + [state])
   }
 
-  function concretePathFragmentTillBranchOrExit(prog: Program, conc_path: ConcretePath) : (r: ConcretePath)
-    requires forall idx: nat :: idx < |conc_path.path| ==> 0 <= conc_path.path[idx].pc <= |prog.stmts|
-    decreases |conc_path.path|
-  {
-    if |conc_path.path| == 0 then
-      ConcretePath([])
-    else if conc_path.path[0].pc == |prog.stmts| then
-      ConcretePath([])
-    else
-      var pc : nat := conc_path.path[0].pc;
-      assert pc < |prog.stmts|;
-
-      var cur_inst := prog.stmts[pc];
-      match cur_inst {
-        case JmpZero(_, _) => ConcretePath([])
-        case Assign(_, _) => 
-          var rest_of_path := concretePathFragmentTillBranchOrExit(prog, ConcretePath(conc_path.path[1..]));
-          ConcretePath([conc_path.path[0]] + rest_of_path.path)
-      }
+  predicate program_path_branch_free(prog: Program, pc: nat, length: nat) {
+    forall pc' :: pc <= pc' < pc + length ==> !is_branch_instruction(prog, pc')
   }
 
-  //predicate equalPCValues
+  predicate abstract_path_branch_free(prog: Program, path: AbstractPath) {
+    forall idx :: 0 <= idx < |path.path| ==> !is_branch_instruction(prog, path.path[idx].pc)
+  }
 
-  // Returns the path along with whether the last instructucion was a branch or an exit
-  function exploreTillBranchOrExit(prog: Program, inst_idx: nat, abs_state: AbstractState) : (AbstractPath, InstructionType)
+  lemma exploreTillBranchOrExit_pc_ok(prog: Program, pc: nat, abs_state: AbstractState)
     requires |prog.stmts| > 0
-    requires inst_idx <= |prog.stmts|
+    requires pc <= |prog.stmts|
     requires programWellFormed(prog)
     requires has_valid_jump_targets(prog.stmts, 0)
+
+    ensures forall p: ConcretePath :: is_basic_block_fragment(prog, p) && state_included(p.path[0].state, abs_state) ==> 
+      |exploreTillBranchOrExit(prog, p.path[0].pc, abs_state).0.path| == |p.path|
+  {
+    assert forall p: ConcretePath :: is_basic_block_fragment(prog, p) && state_included(p.path[0].state, abs_state) ==> 
+      |exploreTillBranchOrExit(prog, p.path[0].pc, abs_state).0.path| > 0;
+    assert forall p: ConcretePath :: is_basic_block_fragment(prog, p) && state_included(p.path[0].state, abs_state) ==> 
+      exploreTillBranchOrExit(prog, p.path[0].pc, abs_state).0.path[0].pc == p.path[0].pc;
+  }
+
+  // Returns the path along with whether the last instructucion was a branch or an exit
+  function exploreTillBranchOrExit(prog: Program, pc: nat, abs_state: AbstractState) : (r : (AbstractPath, InstructionType))
+    requires |prog.stmts| > 0
+    requires pc <= |prog.stmts|
+    requires programWellFormed(prog)
+    requires has_valid_jump_targets(prog.stmts, 0)
+
     // Make sure that we stay within bounds of the program
-    ensures inst_idx < |prog.stmts| ==> inst_idx + |exploreTillBranchOrExit(prog, inst_idx, abs_state).0.path| <= |prog.stmts|
-    ensures inst_idx < |prog.stmts| && prog.stmts[inst_idx].JmpZero? ==> |exploreTillBranchOrExit(prog, inst_idx, abs_state).0.path| == 0
-    ensures (forall i :: 0 <= i < |exploreTillBranchOrExit(prog, inst_idx, abs_state).0.path| < |prog.stmts| ==> 0 <= exploreTillBranchOrExit(prog, inst_idx, abs_state).0.path[i].pc < |prog.stmts|)
+    ensures pc_in_bounds(prog, pc) ==> pc_offset_in_bounds_or_at_end(prog, pc, |r.0.path|)
+    ensures (forall idx :: in_bounds_path(idx, r.0.path) ==> r.0.path[idx].pc == pc + idx)
 
     // Make sure that instruction following the path is a branch instruction and everything in between is not a branch
-    ensures inst_idx + |exploreTillBranchOrExit(prog, inst_idx, abs_state).0.path| < |prog.stmts| ==>
-              prog.stmts[inst_idx + |exploreTillBranchOrExit(prog, inst_idx, abs_state).0.path|].JmpZero? &&
-              exploreTillBranchOrExit(prog, inst_idx, abs_state).1.BranchInstruction? &&
-              (forall i :: inst_idx <= i < inst_idx + |exploreTillBranchOrExit(prog, inst_idx, abs_state).0.path| ==> !prog.stmts[i].JmpZero?) &&
-              (forall i :: 0 <= i < |exploreTillBranchOrExit(prog, inst_idx, abs_state).0.path| ==> !prog.stmts[exploreTillBranchOrExit(prog, inst_idx, abs_state).0.path[i].pc].JmpZero?)
+    ensures pc_offset_in_bounds(prog, pc, |r.0.path|) ==>
+              is_branch_instruction(prog, pc + |r.0.path|) &&
+              r.1.BranchInstruction? &&
+              program_path_branch_free(prog, pc, |r.0.path|) &&
+              abstract_path_branch_free(prog, r.0)
 
     // Make sure that we return a FunctionExit on an actual function exit and everything in between is not a branch
-    ensures inst_idx + |exploreTillBranchOrExit(prog, inst_idx, abs_state).0.path| == |prog.stmts| ==>
-              exploreTillBranchOrExit(prog, inst_idx, abs_state).1.FunctionExit? && (forall i :: inst_idx <= i < |prog.stmts| ==> !prog.stmts[i].JmpZero?) &&
-              (forall i :: 0 <= i < |exploreTillBranchOrExit(prog, inst_idx, abs_state).0.path| < |prog.stmts| ==> !prog.stmts[exploreTillBranchOrExit(prog, inst_idx, abs_state).0.path[i].pc].JmpZero?)
-    
-    /*ensures forall conc_state: E.State :: 
-      (state_included(conc_state, abs_state) &&
-        verifierExploreConcretePath(prog, inst_idx, conc_state, |prog.stmts| + 1).Some?) ==> (
-          ( var r := verifierExploreConcretePath(prog, inst_idx, conc_state, |prog.stmts| + 1).v; &&
-            |concretePathFragmentTillBranchOrExit(prog, r).path| == |exploreTillBranchOrExit(prog, inst_idx, abs_state).0.path| )
-        )*/
+    ensures pc_at_end(prog, pc + |r.0.path|) ==>
+              r.1.FunctionExit? && 
+              program_path_branch_free(prog, pc, |r.0.path|) &&
+              abstract_path_branch_free(prog, r.0)
 
-    decreases |prog.stmts| - inst_idx
+    decreases |prog.stmts| - pc
   {
     var empty_path : AbstractPath := AbstractPath([]);
 
-    if inst_idx == |prog.stmts| then
-      assert |empty_path.path| == 0;
+    if pc == |prog.stmts| then
       (empty_path, FunctionExit)
     else
 
-      var cur_inst := prog.stmts[inst_idx];
+      var cur_inst := prog.stmts[pc];
 
       match cur_inst {
         case JmpZero(_, _) => (empty_path, BranchInstruction)
         case Assign(r, e) =>
-          var v := AbstractEval.expr_eval(abs_state, e);
-          var new_state := AbstractEval.update_state(abs_state, r, v);
+  
+          var new_state := AbstractEval.stmt_eval(abs_state, cur_inst);
           
           //assert forall conc_state: E.State :: state_included(conc_state, abs_state) ==> state_included(conc_state, new_state);
 
-          assert inst_idx < |prog.stmts|;
-          var path_state := AbstractPathState(new_state, inst_idx, []);
+          assert pc < |prog.stmts|;
+          assert new_state.1 == {1};
 
-          var rest_of_path := exploreTillBranchOrExit(prog, inst_idx + 1, new_state);
+          var path_state := AbstractPathState(new_state.0, pc, []);
+
+          var rest_of_path := exploreTillBranchOrExit(prog, pc + 1, new_state.0);
           (AbstractPath([path_state] + rest_of_path.0.path), rest_of_path.1)
       }
 
@@ -419,43 +141,6 @@ module SimpleVerifierAnalysis {
     stmt.JmpZero?
   }
 
-  predicate equalPathBasicBlockPCValues(prog: Program, abs_path: AbstractPath, concrete_path: ConcretePath)
-  {
-    forall pc: nat :: (0 <= pc < |abs_path.path|) && (0 <= pc < |concrete_path.path|) ==> abs_path.path[pc].pc == concrete_path.path[pc].pc
-  }
-
-  // With fuel = |prog.stmts| + 1 we are guaranteed to hit a branch or a program exit (return)
-  predicate concretePathReachesValidBasicBlock(prog: Program, pc: nat, conc_state: E.State)
-    requires |prog.stmts| > 0
-    requires pc <= |prog.stmts|
-    requires programWellFormed(prog)
-    requires has_valid_jump_targets(prog.stmts, 0)
-  {
-    verifierExploreConcretePath(prog, pc, conc_state, |prog.stmts| + 1).Some?
-  }
-
-  function unwrap_path(path: Option<ConcretePath>): ConcretePath
-    requires path.Some?
-  {
-    match path {
-      case Some(p) => p
-    }
-  }
-
-  // exploreTillBranchOrExit respects the program pc values in a basic block defined by verifierExploreConcretePath
-  lemma exploreTillBranchOrExitRespectsBasicBlock(prog: Program, abs_state: AbstractState, conc_state: E.State, pc: nat)
-    requires pc < |prog.stmts|
-    requires state_included(conc_state, abs_state)
-    requires has_valid_jump_targets(prog.stmts, 0)
-    // ensures forall pc : nat :: (pc < |prog.stmts|) && (concretePathReachesValidBasicBlock(prog, pc, conc_state)) ==>
-    // equalPathBasicBlockPCValues(prog, exploreTillBranchOrExit(prog, pc, abs_state).0,
-    // unwrap_path(verifierExploreConcretePath(prog, pc, conc_state, |prog.stmts| + 1)))
-    ensures |exploreTillBranchOrExit(prog, pc, abs_state).0.path| == |exploreTillBranchOrExitConcrete(prog, pc, conc_state).path|
-  {
-    // assert pc != |prog.stmts| ==> exploreTillBranchOrExit(prog, pc, abs_state).0.path[0].pc == exploreTillBranchOrExitConcrete(prog, pc, conc_state).path[0].pc;
-    //var conc_path := verifierExploreConcretePath(prog, pc, conc_state, |prog.stmts| + 1);
-    //assert conc_path.Some? ==> exists pc: nat :: pc < |unwrap_path(conc_path).path| && prog.stmts[unwrap_path(conc_path).path[pc].pc].JmpZero?;
-  }
 
   // Each sequence on the stack is a valid path --> need to abstract eval and real eval the path
 
@@ -573,291 +258,10 @@ module SimpleVerifierAnalysis {
           ret := AnalysisResult(ret.paths + [concatPaths(cur_path, path.0)]);
       }
 
-      // Reached an exit, pop from the worklist
-      /*if branch_or_exit_idx >= |prog.stmts| || |path.0.path| == 0 {
-        // Add path to analysis result
-        ret := AnalysisResult(ret.paths + [concatPaths(cur_path, path.0)]);
-
-        if |worklist| == 0 {
-          // We are done with the exploration
-          break;
-        } else {
-          // Pop from the worklist
-          var worklist_top := worklist[|worklist| - 1];
-          prev_inst_idx := worklist_top.prev_inst_idx;
-          cur_inst_idx := worklist_top.inst_idx;
-          cur_path := worklist_top.path;
-          cur_state := worklist_top.verifier_state;
-          worklist := worklist[..|worklist| - 1];
-        }
-
-      } else {
-  predicate path_state_included(path_state: P
-          // Should happen only if we ran out of fuel for exploration
-          case Assign(_, _) =>
-            ret := AnalysisResult(ret.paths + [concatPaths(cur_path, path.0)]);
-          case JmpZero(_ , offset) =>
-            // We ended at a branch, we should push the taken branch onto the stack and continue exploring the not taken branch
-          has_valid_jump_targets_ok(prog.stmts);
-          assert 0 <= branch_or_exit_idx as int + offset as int <= |prog.stmts|;
-
-
-          var not_taken_pc := branch_or_exit_idx + 1;
-          var taken_pc := branch_or_exit_idx as int + offset as int;
-
-          // The abstract state at the branch instruction is the same as that of the previous (non-branching) instruction
-          var branch_abs_state := AbstractPathState(path.0.path[|path.0.path| - 1].state, branch_or_exit_idx, [not_taken_pc, taken_pc]);
-          var path_so_far := concatPaths(cur_path, concatPaths(path.0, AbstractPath([branch_abs_state])));
-
-          var last_work_elem := VerifierWorkElem(branch_or_exit_idx, taken_pc, branch_abs_state, path_so_far);
-          worklist := worklist + [last_work_elem];
-
-          // Continue exploring the not taken branch
-          cur_inst_idx := not_taken_pc;
-          prev_inst_idx := branch_or_exit_idx;
-          cur_path := path_so_far;
-
-        }
-
-      }*/
-
-      // Decrement 1 to ensure termination
       fuel := fuel - |path.0.path| - 1;
     }
 
     return ret;
   }
-
-  // TODO: connect exploreTillBranchOrExit to this
-  function exploreTillBranchOrExitConcrete(prog: Program, pc: nat, conc_state: E.State): (r: ConcretePath)
-    requires |prog.stmts| > 0
-    requires pc <= |prog.stmts|
-    requires programWellFormed(prog)
-    requires has_valid_jump_targets(prog.stmts, 0)
-
-    decreases |prog.stmts| - pc
-    ensures (var t := exploreTillBranchOrExitConcrete(prog, pc, conc_state);
-              && var u := verifierExploreConcretePathFuel(prog, pc, conc_state, |t.path|);
-              && |u.path| == |t.path|)
-    ensures (var t := exploreTillBranchOrExitConcrete(prog, pc, conc_state);
-              && var u := verifierExploreConcretePathFuel(prog, pc, conc_state, |t.path|);
-              && forall idx: nat :: idx < |u.path| ==> 
-                                (t.path[idx].pc == u.path[idx].pc)
-                                && state_equal(t.path[idx].state, u.path[idx].state))
-  {
-    var empty_path : ConcretePath := ConcretePath([]);
-    var cur_pc := pc;
-    var cur_state := conc_state;
-    var ret := ConcretePath([PathState(cur_state, cur_pc)]);
-
-    if pc == |prog.stmts| then
-      assert |empty_path.path| == 0;
-      //ConcretePath([PathState(conc_state, pc)])
-      ConcretePath([])
-    else
-
-      var cur_inst := prog.stmts[pc];
-
-      match cur_inst {
-        case JmpZero(_, _) => empty_path
-        case Assign(r, e) =>
-          match E.expr_eval(conc_state, e) {
-            case Some(v) => 
-              var new_state := E.update_state(conc_state, r, v);
-          
-              //assert forall conc_state: E.State :: state_included(conc_state, abs_state) ==> state_included(conc_state, new_state);
-
-              assert pc < |prog.stmts|;
-              //var path_state := PathState(new_state, pc);
-
-              var rest_of_path := exploreTillBranchOrExitConcrete(prog, pc + 1, new_state);
-              ConcretePath(ret.path + rest_of_path.path)
-            case None =>
-              ConcretePath([PathState(conc_state, pc)])
-          }
-      }
-  }
-
-  // Concrete path exploration returning a trace of a concrete path whose length is bounded by fuel
-  function verifierExploreConcretePathFuel(prog: Program, pc: nat, initial_conc_state: E.State, fuel: nat) : (r: ConcretePath)
-    requires fuel >= 0
-    requires |prog.stmts| > 0
-    requires pc <= |prog.stmts|
-    requires programWellFormed(prog)
-    requires has_valid_jump_targets(prog.stmts, 0)
-    ensures (var ret := r;
-              && ((|ret.path| > 0) ==> (ret.path[0].pc <= |prog.stmts|))
-              && (forall idx: nat :: idx < |ret.path| ==> 0 <= ret.path[idx].pc <= |prog.stmts|))
-    ensures (var t := verifierExploreConcretePath(prog, pc, initial_conc_state, fuel);
-              && var u := verifierExploreConcretePathFuel(prog, pc, initial_conc_state, fuel);
-              && t.Some? ==> (|t.v.path| == |u.path|))
-
-    // Prove that verifierExploreConcretePathFuel returns a trace of an actual terminating program state bounded in length by fuel
-    ensures (var t := verifierExploreConcretePath(prog, pc, initial_conc_state, fuel);
-              && var u := verifierExploreConcretePathFuel(prog, pc, initial_conc_state, fuel);
-              && t.Some? ==> (forall idx: nat :: idx < |t.v.path| ==> 
-                                t.v.path[idx].pc == u.path[idx].pc 
-                                && state_equal(t.v.path[idx].state, u.path[idx].state)))
-    decreases fuel
-  {
-    var cur_pc := pc;
-    var cur_state := initial_conc_state;
-    var ret := ConcretePath([PathState(cur_state, cur_pc)]);
-    var fuel := fuel;
-
-    if cur_pc == |prog.stmts| then
-      assert forall idx: nat :: idx < |ret.path| ==> ret.path[idx].pc <= |prog.stmts|;
-      //ret
-      ConcretePath([])
-    else if fuel == 0 then
-      //ret
-      ConcretePath([])
-    else
-
-      var cur_inst := prog.stmts[cur_pc];
-      match cur_inst {
-        case Assign(r, e) =>
-          var e' := E.expr_eval(cur_state, e);
-          match e' {
-            case Some(v) =>
-              var cur_state := E.update_state(cur_state, r, v);
-              var cur_pc := cur_pc + 1;
-              assert cur_pc <= |prog.stmts|;
-              var rest_of_path := verifierExploreConcretePathFuel(prog, cur_pc, cur_state, fuel - 1);
-              assert forall idx: nat :: idx < |ret.path| ==> ret.path[idx].pc <= |prog.stmts|;
-
-              assert |ret.path| == 1;
-              assert ret.path[0].pc <= |prog.stmts|;
-              //assert rest_of_path.path[0].pc == cur_pc;
-              var ret := ConcretePath(ret.path + rest_of_path.path);
-              
-              assert forall idx: nat :: idx < |rest_of_path.path| ==> rest_of_path.path[idx].pc <= |prog.stmts|;
-              ret
-
-            case None =>
-              // Return a partial path even if there is an error state
-              var ret := ConcretePath(ret.path);
-              assert ret.path[0].pc <= |prog.stmts|;
-              ret
-          }
-        case JmpZero(r, offset) =>
-          var jmp := if cur_state(r) == 0 then offset else 1;
-          has_valid_jump_targets_ok(prog.stmts);
-          assert cur_pc + jmp as int <= |prog.stmts|;
-          var cur_pc := cur_pc + jmp as int;
-          assert cur_pc <= |prog.stmts|;
-          var rest_of_path := verifierExploreConcretePathFuel(prog, cur_pc, cur_state, fuel - 1);
-
-
-          //assert rest_of_path.path[0].pc == cur_pc;
-          assert |ret.path| == 1;
-          assert ret.path[0].pc <= |prog.stmts|;
-              // assert forall idx: nat :: (idx < |conc_path.path|)
-              //                           && (idx + 1 < |conc_path.path|)
-              //                           && (0 <= conc_path.path[idx].pc < |prog.stmts|)
-              //                           && (prog.stmts[conc_path.path[idx].pc].Assign?)
-              //                           ==> conc_path.path[idx + 1].pc == conc_path.path[idx].pc + 1;
-          var ret := ConcretePath(ret.path + rest_of_path.path);
-          ret
-
-      }
-
-  }
-
-  // Concrete path exploration
-  // Return None if we run out of fuel
-  function verifierExploreConcretePath(prog: Program, pc: nat, initial_conc_state: E.State, fuel: nat) : (r:Option<ConcretePath>)
-    requires fuel >= 0
-    requires |prog.stmts| > 0
-    requires pc <= |prog.stmts|
-    requires programWellFormed(prog)
-    requires has_valid_jump_targets(prog.stmts, 0)
-    ensures r.Some? ==>
-              (var ret := r.v;
-               //&& |ret.path| > 0
-               //&& ret.path[0].pc <= |prog.stmts|
-               && forall idx: nat :: idx < |ret.path| ==> 0 <= ret.path[idx].pc <= |prog.stmts|)
-    
-    //  (forall idx: nat :: idx < |unwrap_path(verifierExploreConcretePath(prog, pc, initial_conc_state, fuel)).path| ==>
-    //    unwrap_path(verifierExploreConcretePath(prog, pc, initial_conc_state, fuel)).path[idx].pc <= |prog.stmts|
-    //  )
-    decreases fuel
-  {
-    var cur_pc := pc;
-    var cur_state := initial_conc_state;
-    var ret := ConcretePath([PathState(cur_state, cur_pc)]);
-    var fuel := fuel;
-
-    if cur_pc == |prog.stmts| then
-      assert forall idx: nat :: idx < |ret.path| ==> ret.path[idx].pc <= |prog.stmts|;
-      //Some(ret)
-      // TODO: Think about whether we need to return the state when pc = |prog.stmts| (the line commented above)
-      // If yes, then change the same line for all the functions above this
-      Some(ConcretePath([]))
-    else if fuel == 0 then
-      None
-    else
-
-      var cur_inst := prog.stmts[cur_pc];
-      match cur_inst {
-        case Assign(r, e) =>
-          var e' := E.expr_eval(cur_state, e);
-          match e' {
-            case Some(v) =>
-              var cur_state := E.update_state(cur_state, r, v);
-              var cur_pc := cur_pc + 1;
-              assert cur_pc <= |prog.stmts|;
-              assert cur_pc == |prog.stmts| ==> verifierExploreConcretePath(prog, cur_pc, cur_state, fuel - 1).Some?;
-              var rest_of_path := verifierExploreConcretePath(prog, cur_pc, cur_state, fuel - 1);
-              assert forall idx: nat :: idx < |ret.path| ==> ret.path[idx].pc <= |prog.stmts|;
-              match rest_of_path {
-                case Some(conc_path) =>
-                  assert |ret.path| == 1;
-                  assert ret.path[0].pc <= |prog.stmts|;
-                  //assert conc_path.path[0].pc == cur_pc;
-                  var ret := ConcretePath(ret.path + conc_path.path);
-                  assert rest_of_path.Some?;
-                  assert forall idx: nat :: idx < |conc_path.path| ==> conc_path.path[idx].pc <= |prog.stmts|;
-                  Some(ret)
-                case None =>
-                  None
-              }
-            case None =>
-              // Return a partial path even if there is an error state
-              var ret := ConcretePath(ret.path);
-              assert ret.path[0].pc <= |prog.stmts|;
-              Some(ret)
-          }
-        case JmpZero(r, offset) =>
-          var jmp := if cur_state(r) == 0 then offset else 1;
-          has_valid_jump_targets_ok(prog.stmts);
-          assert cur_pc + jmp as int <= |prog.stmts|;
-          var cur_pc := cur_pc + jmp as int;
-          assert cur_pc <= |prog.stmts|;
-          var rest_of_path := verifierExploreConcretePath(prog, cur_pc, cur_state, fuel - 1);
-          match rest_of_path {
-            case Some(conc_path) =>
-              //assert conc_path.path[0].pc == cur_pc;
-              assert |ret.path| == 1;
-              assert ret.path[0].pc <= |prog.stmts|;
-              // assert forall idx: nat :: (idx < |conc_path.path|)
-              //                           && (idx + 1 < |conc_path.path|)
-              //                           && (0 <= conc_path.path[idx].pc < |prog.stmts|)
-              //                           && (prog.stmts[conc_path.path[idx].pc].Assign?)
-              //                           ==> conc_path.path[idx + 1].pc == conc_path.path[idx].pc + 1;
-              var ret := ConcretePath(ret.path + conc_path.path);
-              Some(ret)
-            case None =>
-              None
-          }
-      }
-
-  }
-
-  //lemma concretePathContainedInAbstractPath(prog: Program, initial_conc_state: E.State, initial_abstract_state: AbstractState, fuel: nat)
-  //  requires state_included(initial_conc_state, initial_abstract_state)
-  //{
-  //  assert |verifierExploreConcretePath(prog, 0, initial_conc_state, fuel).path| == |verifierExplorePaths(prog, initial_abstract_state, fuel).path|;
-  //}
 
 }
