dafny/abstract-interpreter/helpers.dfy
@@ -1,8 +1,10 @@
 include "BoundedInts.dfy"
+include "SimpleVerifier.dfy"
 
 module helpers {
 
   import opened BoundedInts
+  import opened Lang
 
   function signed_add64(a: uint64, b: uint64): uint64 {
     (((a as int) + (b as int)) % 0x1_00000000_00000000) as uint64
@@ -29,5 +31,37 @@ module helpers {
       a as uint32
   }
 
+  predicate pc_in_bounds(prog: Program, pc: int) {
+    0 <= pc < |prog.stmts|
+  }
+
+  predicate pc_at_end(prog: Program, pc: int) {
+    pc == |prog.stmts|
+  }
+
+  predicate pc_in_bounds_or_at_end(prog: Program, pc: int) {
+    pc_in_bounds(prog, pc) || pc_at_end(prog, pc)
+  }
+
+  predicate pc_offset_in_bounds_or_at_end(prog: Program, pc: nat, offset: nat) {
+    pc_in_bounds_or_at_end(prog, pc + offset)
+  }
+
+  predicate pc_offset_in_bounds(prog: Program, pc: nat, offset: nat) {
+    pc_in_bounds(prog, pc + offset)
+  }
+
+  predicate in_bounds_path<T>(i: int, path: seq<T>) {
+    0 <= i < |path|
+  }
+
+  predicate is_branch_instruction(prog: Program, pc: nat) {
+    prog.stmts[pc].JmpZero?
+  }
+
+  // pc in [start, end)
+  predicate pc_in_range(pc: nat, start: nat, end: nat) {
+    start <= pc < end
+  }
 
 }
