dafny/abstract-interpreter/ConcreteExecution.dfy
@@ -1,0 +1,75 @@
+include "SimpleVerifier.dfy"
+include "helpers.dfy"
+
+module ConcreteExecution {
+    import opened Lang
+    import opened ConcreteEval
+    import opened Ints
+    import opened helpers
+
+    datatype PathState = PathState(state: ConcreteEval.State, pc: nat)
+
+    datatype ConcretePath = ConcretePath(path: seq<PathState>)
+
+    function init_conc_reg_state(r: Reg): u32 {
+        0
+    }
+
+    function initial_concrete_state(stmt: Stmt): PathState {
+        PathState(init_conc_reg_state, 0)
+    }
+
+    predicate state_equal(s1: ConcreteEval.State, s2: ConcreteEval.State) {
+        forall r : Reg :: s1(r) == s2(r)
+    }
+
+    predicate stmt_step_valid(prog: Program, initial_state: PathState, final_state: PathState)
+    {
+        var init_pc := initial_state.pc;
+        var final_pc := final_state.pc;
+
+        if pc_at_end(prog, init_pc) then
+            // Check whether we stay at the same state
+            pc_at_end(prog, final_pc) && 
+                state_equal(initial_state.state, final_state.state)
+        else if pc_in_bounds(prog, init_pc) then
+            var stmt := prog.stmts[init_pc];
+            match ConcreteEval.stmt_step(initial_state.state, stmt) {
+                case Some((fin, offset)) =>
+                    (init_pc + offset == final_pc) && 
+                        state_equal(fin, final_state.state) &&
+                        pc_in_bounds_or_at_end(prog, final_pc)
+                case None => false
+            }
+        else
+            // !pc_in_bounds(prog, init_pc) && !(pc_at_end(prog, pc))
+            // pc points to space
+            false
+    }
+
+    predicate is_valid_path(prog: Program, path: ConcretePath) {
+        if |path.path| == 0 then
+            true
+        else if |path.path| == 1 then
+            pc_in_bounds_or_at_end(prog, path.path[0].pc)
+        else
+            stmt_step_valid(prog, path.path[0], path.path[1]) && 
+                is_valid_path(prog, ConcretePath(path.path[1..]))
+    }
+
+    predicate concrete_path_branch_free(prog: Program, path: ConcretePath) {
+        forall idx :: 0 <= idx < |path.path| ==> !is_branch_instruction(prog, path.path[idx].pc)
+    }
+
+    predicate is_basic_block_fragment(prog: Program, path: ConcretePath) {
+        |path.path| > 0 &&
+        is_valid_path(prog, path) && 
+        pc_in_bounds(prog, path.path[0].pc) &&
+        !is_branch_instruction(prog, path.path[0].pc) &&
+        concrete_path_branch_free(prog, path) &&
+        (   pc_at_end(prog, path.path[|path.path| - 1].pc + 1)  ||
+            (   pc_in_bounds(prog, path.path[|path.path| - 1].pc + 1) &&
+                is_branch_instruction(prog, path.path[|path.path| - 1].pc + 1)  )
+        )
+    }
+}
